\section{Intersection of Straight Lines}
Let $\vp, \vq \in \R^3$ be two position vectors and $\vv, \vw \in \R^3$
directional vectors. Straight lines are described by the following equations:
\begin{equation}
g(\lambda) = \vp + \lambda \vv \nn
\end{equation}
and
\begin{equation}
h(\mu) = \vq + \mu \vw. \nn
\end{equation}
Points along straight lines can be specified by fixed $\lambda$ and $\mu$
repectively. The distance of two points, the first within $g(\lambda)$, the
second within $h(\mu)$, can be written as:
\begin{equation*}
\varrho(\lambda, \mu) = \vnorm{g(\lambda) - h(\mu)}_2
	= \vnorm{\vp - \vq + \lambda \vv - \mu \vw}_2
	= \sqrt{\underbrace{\sum_{i=1}^3
		\left(p_i - q_i + \lambda v_i - \mu w_i \right)^2}_{:= f(\lambda,\mu)}}
\end{equation*}
The distance function can only be minimal if
\begin{equation*}
\nabla \varrho (\lambda, \mu) = \left(
	\dfrac{\partial \varrho}{\partial \lambda} (\lambda, \mu),
	\dfrac{\partial \varrho}{\partial \mu} (\lambda, \mu)
	\right)
	= \left(
	\dfrac{\partial f}{\partial \lambda}(\lambda, \mu)
		\dfrac{1}{\sqrt{f(\lambda, \mu)}},
	\dfrac{\partial f}{\partial \mu}(\lambda, \mu)
		\dfrac{1}{\sqrt{f(\lambda, \mu)}} \right) = 0.
\end{equation*}
\begin{align*}
f(\lambda, \mu)
	&= \sum_{i=1}^3 \left(p_i - q_i + \lambda v_i - \mu w_i \right)^2 \nn \\
	&= \sum_{i=1}^3 \left( p_i^2 - p_i q_i + \lambda p_i v_i - \mu p_i w_i \right)
		+ \left(q_i p_i - q_i^2 + \lambda q_i v_i - \mu q_i w_i \right) \nn \\
		&\qquad + \left(\lambda p_i v_i - \lambda q_i v_i + \lambda^2 v_i^2 - \lambda \mu v_i w_i \right)
		+ \left(\mu p_i w_i - \mu q_i w_i + \lambda \mu v_i w_i - \mu^2 w_i^2 \right) \nn \\
	&= \sum_{i=1}^3 p_i^2 + q_i^2 - 2 p_i q_i + 2 \lambda p_i v_i
		- 2 \lambda q_i v_i - 2 \mu p_i w_i + 2 \mu w_i q_i
		- 2 \lambda \mu v_i w_i + \lambda^2 v_i^2 + \mu^2 w_i^2 \\
\dfrac{\partial f}{\partial \lambda}(\lambda, \mu)
	&= 2 \sum_{i=1}^3 p_i v_i - q_i v_i - \mu v_i w_i + v_i^2 \lambda \\
\dfrac{\partial f}{\partial \mu}(\lambda, \mu)
	&= 2 \sum_{i=1}^3 - p_i w_i + q_i w_i - \lambda v_i w_i + w_i^2 \mu
\end{align*}
The terms
\begin{equation*}
\dfrac{\partial f}{\partial \lambda}(\lambda, \mu)
	\dfrac{1}{\sqrt{f(\lambda, \mu)}}
\quad \textnormal{and} \quad
\dfrac{\partial f}{\partial \mu}(\lambda, \mu)
	\dfrac{\partial f}{\partial \mu}(\lambda, \mu)
\end{equation*}
vanishs, if
\begin{equation*}
\sum_{i=1}^3 p_i v_i - q_i v_i - \mu v_i w_i + v_i^2 \lambda = 0
\quad \textnormal{and} \quad
\sum_{i=1}^3 - p_i w_i + q_i w_i - \lambda v_i w_i + w_i^2 \mu = 0
\end{equation*}
holds. It results the following system of linear equations
\begin{equation*}
\begin{pmatrix}
\sum_{i=1}^3 v_i^2 & - \sum_{i=1}^3 v_i w_i \\
- \sum_{i=1}^3 w_i v_i & \sum_{i=1}^3 w_i^2 \\
\end{pmatrix}
\begin{pmatrix}
\lambda \\ \mu
\end{pmatrix}
=
\begin{pmatrix}
\sum_{i=1}^3 v_i (q_i - p_i) \\
\sum_{i=1}^3 w_i (p_i - q_i)
\end{pmatrix}
\end{equation*}
